update

lib/Lib.Circuits.fst
@@ -56,13 +56,14 @@ let l1 : bar =
 
 let l1xM_def (m:nat) : Lemma (xNxM l1.xN m == x1xM bool m) [SMTPat (xNxM l1.xN m)] = ()
 
+noextract
 val circuit_def (#m #p:nat) (circ:circuit m p) (#lN:bar) (x:xNxM lN.xN m) (i:nat{i<p}) : lN.xN.t
 #push-options "--ifuel 1"
 let rec circuit_def #m #p circ #lN x i =
   let Cons circ g = circ in
   if i=p-1 then
     match g with
-    | Input j -> index x j
+    | Input j -> index j x
     | Zeros -> (_).zeros_
     | Ones -> (_).ones_
     | And a b -> (_).and_ (circuit_def circ x a) (circuit_def circ x b)
@@ -132,14 +133,16 @@ let rec sliceable_circuit_lemma #m #p circ #lN x i j =
    sliceable_circuit_lemma circ x i j
 #pop-options
 
+noextract
 val circuit_spec (#m #m':nat) (circ:circuit m m') (lN:bar) (x:xNxM lN.xN m) : xNxM lN.xN m'
 let circuit_spec circ _ x = xNxM_mk _ _ (circuit_def circ x)
 
 val circuit_spec_lemma (#m #m':nat) (circ:circuit m m') (lN:bar) (x:xNxM lN.xN m) (i:nat{i<m'}) :
-  Lemma (index (circuit_spec circ lN x) i == circuit_def circ x i)
-  [SMTPat (index (circuit_spec circ lN x) i)]
+  Lemma (index i (circuit_spec circ lN x) == circuit_def circ x i)
+  [SMTPat (index i (circuit_spec circ lN x))]
 let circuit_spec_lemma circ x lN i = ()
 
+noextract
 val circuit_spec' (#m #p:nat) (circ:circuit m p) (lN:bar) (x:xNxM lN.xN m) : (y:xNxM lN.xN p{y == circuit_spec circ lN x})
 #push-options "--fuel 1 --ifuel 1"
 let rec circuit_spec' #m #p circ lN x =
@@ -150,13 +153,13 @@ let rec circuit_spec' #m #p circ lN x =
     let y : xNxM lN.xN (p-1) = circuit_spec' circ' lN x in
     let w : (w:lN.xN.t{w == circuit_def circ x (p-1)}) =
       match g with
-      | Input j -> index x j
+      | Input j -> index j x
       | Ones -> (_).ones_
       | Zeros -> (_).zeros_
-      | Xor a b -> (_).xor_ (index y a) (index y b)
-      | And a b -> (_).and_ (index y a) (index y b)
-      | Or a b -> (_).or_ (index y a) (index y b)
-      | Not a -> (_).not_ (index y a)
+      | Xor a b -> (_).xor_ (index a y) (index b y)
+      | And a b -> (_).and_ (index a y) (index b y)
+      | Or a b -> (_).or_ (index a y) (index b y)
+      | Not a -> (_).not_ (index a y)
     in
     let z : xNxM lN.xN p = ((w <: lN.xN.t), y) in
     assert(w == circuit_def circ x (p-1));
@@ -186,59 +189,59 @@ let circ_st_empty (m:nat) =
 }
 
 type st_monad (b:Type0) (a:Type0) = b -> a * b
-let bind (#b:Type0) (m:st_monad b 'a) (f:'a -> st_monad b 'b) : st_monad b 'b =
+noextract let bind (#b:Type0) (m:st_monad b 'a) (f:'a -> st_monad b 'b) : st_monad b 'b =
 fun s -> let (a, s') = m s in f a s'
-let return (#b:Type0) (x:'a) : st_monad b 'a =
+noextract let return (#b:Type0) (x:'a) : st_monad b 'a =
 fun s -> (x,s)
-let put (#b:Type0) (s:b) : st_monad b unit =
+noextract let put (#b:Type0) (s:b) : st_monad b unit =
 fun _ -> ((),s)
-let get (#b:Type0) : st_monad b b =
+noextract let get (#b:Type0) : st_monad b b =
 fun s -> (s,s)
-let run (#b:Type0) (m:st_monad b 'a) (s:b) : 'a*b = m s
+noextract let run (#b:Type0) (m:st_monad b 'a) (s:b) : 'a*b = m s
 
-let bld_aux (st:circ_st) (g:gate st.m st.p) : circ_st =
+noextract let bld_aux (st:circ_st) (g:gate st.m st.p) : circ_st =
 { m = st.m
 ; p = st.p+1
 ; circ = Cons st.circ g
 }
 
-let bld_zeros : st_monad circ_st nat =
+noextract let bld_zeros : st_monad circ_st nat =
   st <-- get;
   _ <-- put (bld_aux st Zeros);
   return st.p
 
-let bld_ones : st_monad circ_st nat =
+noextract let bld_ones : st_monad circ_st nat =
   st <-- get;
   _ <-- put (bld_aux st Ones);
   return st.p
 
-let bld_input (j:nat) : st_monad circ_st nat =
+noextract let bld_input (j:nat) : st_monad circ_st nat =
   st <-- get;
   _ <-- put (bld_aux st (if j<st.m then Input j else Zeros));
   return st.p
 
-let bld_and (a b:nat) : st_monad circ_st nat =
+noextract let bld_and (a b:nat) : st_monad circ_st nat =
   st <-- get;
   _ <-- put (bld_aux st (if a<st.p && b<st.p then And a b else Zeros));
   return st.p
 
-let bld_xor (a b:nat) : st_monad circ_st nat =
+noextract let bld_xor (a b:nat) : st_monad circ_st nat =
   st <-- get;
   _ <-- put (bld_aux st (if a<st.p && b<st.p then Xor a b else Zeros));
   return st.p
 
-let bld_or (a b:nat) : st_monad circ_st nat =
+noextract let bld_or (a b:nat) : st_monad circ_st nat =
   st <-- get;
   _ <-- put (bld_aux st (if a<st.p && b<st.p then Or a b else Zeros));
   return st.p
 
-let bld_not (a:nat) : st_monad circ_st nat =
+noextract let bld_not (a:nat) : st_monad circ_st nat =
   st <-- get;
   _ <-- put (bld_aux st (if a<st.p then Not a else Zeros));
   return st.p
 
 #push-options "--ifuel 1"
-let rec nth_gate (#m #p:nat) (circ:circuit m p) (i:nat{i<p}) : gate m i =
+noextract let rec nth_gate (#m #p:nat) (circ:circuit m p) (i:nat{i<p}) : gate m i =
   let Cons circ g = circ in
   if i=p-1 then g else nth_gate circ i
 #pop-options
@@ -265,7 +268,7 @@ let rec nth_gate_eq_intro (#m #p:nat) (circ1 circ2:circuit m p) :
 #pop-options
 
 #push-options "--fuel 1"
-let rec circuit_of_fun (#m #p:nat) (f:(i:nat{i<p} -> gate m i)) : (circ:circuit m p{forall (i:nat{i<p}). nth_gate circ i == f i}) =
+noextract let rec circuit_of_fun (#m #p:nat) (f:(i:nat{i<p} -> gate m i)) : (circ:circuit m p{forall (i:nat{i<p}). nth_gate circ i == f i}) =
   if p=0 then Empty else Cons (circuit_of_fun f) (f (p-1))
 #pop-options
 
@@ -280,18 +283,85 @@ let circuit_def_lemma #m #p circ g #lN x i = ()
 #pop-options
 
 #push-options "--fuel 1 --ifuel 1"
-let rec nth_gate_zeros (#m #p:nat) (circ:circuit m p) (#lN:bar) (inputs:xNxM lN.xN m) (i:nat{i<p}) :
-  Lemma (requires nth_gate circ i == Zeros) (ensures circuit_def circ inputs i == (_).zeros_)
+let rec nth_gate_zeros (#m #p:nat) (circ:circuit m p) (#lN:bar) (inputs:xNxM lN.xN m) (i:nat{i<p})
+  : Lemma (requires nth_gate circ i == Zeros) (ensures circuit_def circ inputs i == (_).zeros_)
   =
   if i=p-1 then () else let Cons circ' g = circ in nth_gate_zeros circ' inputs i
 
-let rec nth_gate_ones (#m #p:nat) (circ:circuit m p) (#lN:bar) (inputs:xNxM lN.xN m) (i:nat{i<p}) :
-  Lemma (requires nth_gate circ i == Ones) (ensures circuit_def circ inputs i == (_).ones_)
+let rec nth_gate_ones (#m #p:nat) (circ:circuit m p) (#lN:bar) (inputs:xNxM lN.xN m) (i:nat{i<p})
+  : Lemma (requires nth_gate circ i == Ones) (ensures circuit_def circ inputs i == (_).ones_)
   =
   if i=p-1 then () else let Cons circ' g = circ in nth_gate_ones circ' inputs i
 
-let rec nth_gate_input (#m #p:nat) (circ:circuit m p) (#lN:bar) (inputs:xNxM lN.xN m) (i:nat{i<p}) (j:nat{j<m}) :
-  Lemma (requires nth_gate circ i == Input j) (ensures circuit_def circ inputs i == index inputs j)
+let rec nth_gate_input (#m #p:nat) (circ:circuit m p) (#lN:bar) (inputs:xNxM lN.xN m) (i:nat{i<p})
+  (j:nat{j<m})
+  : Lemma (requires nth_gate circ i == Input j) (ensures circuit_def circ inputs i == index j inputs)
   =
   if i=p-1 then () else let Cons circ' g = circ in nth_gate_input circ' inputs i j
+
+let rec nth_gate_and (#m #p:nat) (circ:circuit m p) (#lN:bar) (inputs:xNxM lN.xN m) (i:nat{i<p})
+  (a:nat{a<i}) (x:(_).t{x==circuit_def circ inputs a}) (b:nat{b<i}) (y:(_).t{y==circuit_def circ inputs b})
+  : Lemma (requires nth_gate circ i == And a b) (ensures circuit_def circ inputs i == (_).and_ x y)
+  =
+  if i=p-1 then () else let Cons circ' g = circ in nth_gate_and circ' inputs i a x b y
+
+let rec nth_gate_xor (#m #p:nat) (circ:circuit m p) (#lN:bar) (inputs:xNxM lN.xN m) (i:nat{i<p})
+  (a:nat{a<i}) (x:(_).t{x==circuit_def circ inputs a}) (b:nat{b<i}) (y:(_).t{y==circuit_def circ inputs b})
+  : Lemma (requires nth_gate circ i == Xor a b) (ensures circuit_def circ inputs i == (_).xor_ x y)
+  =
+  if i=p-1 then () else let Cons circ' g = circ in nth_gate_xor circ' inputs i a x b y
+
+let rec nth_gate_or (#m #p:nat) (circ:circuit m p) (#lN:bar) (inputs:xNxM lN.xN m) (i:nat{i<p})
+  (a:nat{a<i}) (x:(_).t{x==circuit_def circ inputs a}) (b:nat{b<i}) (y:(_).t{y==circuit_def circ inputs b})
+  : Lemma (requires nth_gate circ i == Or a b) (ensures circuit_def circ inputs i == (_).or_ x y)
+  =
+  if i=p-1 then () else let Cons circ' g = circ in nth_gate_or circ' inputs i a x b y
+
+let rec nth_gate_not (#m #p:nat) (circ:circuit m p) (#lN:bar) (inputs:xNxM lN.xN m) (i:nat{i<p})
+  (a:nat{a<i}) (x:(_).t{x==circuit_def circ inputs a})
+  : Lemma (requires nth_gate circ i == Not a) (ensures circuit_def circ inputs i == (_).not_ x)
+  =
+  if i=p-1 then () else let Cons circ' g = circ in nth_gate_not circ' inputs i a x
 #pop-options
+
+noextract let compile_zeros (#m #p:nat) (circ:circuit m p) (#lN:bar) (inputs:xNxM lN.xN m) (i:nat{i<p})
+  : Pure (_).t (requires nth_gate circ i == Zeros) (ensures fun x -> x == circuit_def circ inputs i)
+  = nth_gate_zeros circ inputs i; normalize_term((_).zeros_)
+
+noextract let compile_ones (#m #p:nat) (circ:circuit m p) (#lN:bar) (inputs:xNxM lN.xN m) (i:nat{i<p})
+  : Pure (_).t (requires nth_gate circ i == Ones) (ensures fun x -> x == circuit_def circ inputs i)
+  = nth_gate_ones circ inputs i; normalize_term((_).ones_)
+
+noextract let compile_input (#m #p:nat) (circ:circuit m p) (#lN:bar) (inputs:xNxM lN.xN m) (i:nat{i<p})
+  (j:nat{j<m}) : Pure (_).t (requires nth_gate circ i == Input j) (ensures fun x -> x == circuit_def circ inputs i)
+  =
+  nth_gate_input circ inputs i j;
+  let y = normalize_term(index j) inputs in
+  assume(y == index j inputs);
+  y
+
+noextract let compile_and (#m #p:nat) (circ:circuit m p) (#lN:bar) (inputs:xNxM lN.xN m) (i:nat{i<p})
+  (a:nat{a<i}) (x:(_).t{x==circuit_def circ inputs a})
+  (b:nat{b<i}) (y:(_).t{y==circuit_def circ inputs b})
+  : Pure (_).t (requires nth_gate circ i == And a b) (ensures fun z -> z == circuit_def circ inputs i)
+  = nth_gate_and circ inputs i a x b y; normalize_term((_).and_) x y
+
+noextract let compile_xor (#m #p:nat) (circ:circuit m p) (#lN:bar) (inputs:xNxM lN.xN m) (i:nat{i<p})
+  (a:nat{a<i}) (x:(_).t{x==circuit_def circ inputs a})
+  (b:nat{b<i}) (y:(_).t{y==circuit_def circ inputs b})
+  : Pure (_).t (requires nth_gate circ i == Xor a b) (ensures fun z -> z == circuit_def circ inputs i)
+  = nth_gate_xor circ inputs i a x b y; normalize_term((_).xor_) x y
+
+noextract let compile_or (#m #p:nat) (circ:circuit m p) (#lN:bar) (inputs:xNxM lN.xN m) (i:nat{i<p})
+  (a:nat{a<i}) (x:(_).t{x==circuit_def circ inputs a})
+  (b:nat{b<i}) (y:(_).t{y==circuit_def circ inputs b})
+  : Pure (_).t (requires nth_gate circ i == Or a b) (ensures fun z -> z == circuit_def circ inputs i)
+  = nth_gate_or circ inputs i a x b y; normalize_term((_).or_) x y
+
+noextract let compile_not (#m #p:nat) (circ:circuit m p) (#lN:bar) (inputs:xNxM lN.xN m) (i:nat{i<p})
+  (a:nat{a<i}) (x:(_).t{x==circuit_def circ inputs a})
+  : Pure (_).t (requires nth_gate circ i == Not a) (ensures fun y -> y == circuit_def circ inputs i)
+  = nth_gate_not circ inputs i a x; normalize_term((_).not_) x
+
+noextract let rec circ (n:nat) : circuit 1 (n+1) =
+if n = 0 then Cons Empty (Input 0) else Cons (circ (n-1)) (Xor (n-1) (n-1))
