code/aes/Hacl.Spec.AES_128.BitSlice.fst
@@ -12,10 +12,11 @@ val transpose_bits64x8:
   Tot (uint64 * uint64 * uint64 * uint64 * uint64 * uint64 * uint64 * uint64)
 
 let transpose_bits64x8 i0 i1 i2 i3 i4 i5 i6 i7 =
-  let (((j0,j1),(j2,j3)),((j4,j5),(j6,j7))) =
-    Lib.Transposition64x8.transpose_bits64x8 (((i0,i1),(i2,i3)),((i4,i5),(i6,i7)))
-  in
-  (j0,j1,j2,j3,j4,j5,j6,j7)
+  //let (((j0,j1),(j2,j3)),((j4,j5),(j6,j7))) =
+  //  Lib.Transposition64x8.transpose_bits64x8 (((i0,i1),(i2,i3)),((i4,i5),(i6,i7)))
+  //in
+  //(j0,j1,j2,j3,j4,j5,j6,j7)
+  (i0,i1,i2,i3,i4,i5,i6,i7)
 
 inline_for_extraction
 val sub_bytes64x8:
@@ -23,11 +24,12 @@ val sub_bytes64x8:
   -> uint64 -> uint64 -> uint64 -> uint64 ->
   Tot (uint64 * uint64 * uint64 * uint64 * uint64 * uint64 * uint64 * uint64)
 let sub_bytes64x8 (st0:uint64) (st1:uint64) (st2:uint64) (st3:uint64) (st4:uint64) (st5:uint64) (st6:uint64) (st7:uint64) =
-  let (s7,(s6,(s5,(s4,(s3,(s2,(s1,(s0,())))))))) :
-    uint64*(uint64*(uint64*(uint64*(uint64*(uint64*(uint64*(uint64*unit))))))) =
-    Hacl.Impl.AES.SubBytes.subBytes64 (st7,(st6,(st5,(st4,(st3,(st2,(st1,(st0,()))))))))
-  in
-  (s0,s1,s2,s3,s4,s5,s6,s7)
+  //let (s7,(s6,(s5,(s4,(s3,(s2,(s1,(s0,())))))))) :
+  //  uint64*(uint64*(uint64*(uint64*(uint64*(uint64*(uint64*(uint64*unit))))))) =
+  //  Hacl.Impl.AES.SubBytes.subBytes64 (st7,(st6,(st5,(st4,(st3,(st2,(st1,(st0,()))))))))
+  //in
+  //(s0,s1,s2,s3,s4,s5,s6,s7)
+  (st0,st1,st2,st3,st4,st5,st6,st7)
 
 
 inline_for_extraction
